Core/Infer/TypeSound.lean
@@ -34,7 +34,7 @@ case _ n ih =>
   replace ih := @ih _ _ Γ' h2
   have lem' := Vec.eq_sound h7;
 
-  replace h6 := Vec.seq_sound h6
+  replace h6 := Vec.seq_sound_get_elem h6
   simp only [<-h5.2] at Ks
   simp [SpineTy] at h3;
   let Ts := h3.2.2.2.fst
@@ -69,6 +69,39 @@ case _ y _ ih =>
   simp at h3; exists y.2.1; exists y.2.2.1; exists y.2.2.2; subst h3; rfl
   apply ih h2
 
+theorem pattern_exhaustive_sound (G : GlobalEnv) : (q : Vec String m) -> Query G DataConst.cls q S ->
+  check_exhaustive G S ps = some () -> ∃ i, Query.Match q (ps i) := by sorry
+
+
+theorem data_valid_sound (G : GlobalEnv) :
+  Ty.valid_data c G T = some () ->
+  T.data? c G := by
+intro h
+induction T <;> simp at *
+case _ =>
+  rw[Option.bind_eq_some_iff] at h; rcases h with ⟨h1, h2, h⟩
+  simp at h;
+  simp [Ty.data?, Ty.HeadVariable];
+  exists h1.fst
+case _ =>
+  rw[Option.bind_eq_some_iff] at h; rcases h with ⟨h1, h2, h⟩
+  simp at h;
+  simp [Ty.data?, Ty.HeadVariable];
+  exists h1.fst
+  apply And.intro
+  · exists h1.2;
+  · apply h
+case _ a h _ =>
+  rw[Option.bind_eq_some_iff] at h; rcases h with ⟨h1, h2, h⟩
+  simp at h;
+  simp [Ty.data?, Ty.HeadVariable];
+  exists h1.1
+  replace h2 := Ty.Spine.app_eq.1 h2;
+  rcases h2 with ⟨w, h2, h3⟩;
+  apply And.intro
+  · exists w ++ [a]; exists w;
+  · apply h
+
 theorem infer_type_sound :
   ⊢ G ->
   t.infer_type G Δ Γ = some T ->
@@ -94,36 +127,123 @@ case _ => -- defn
   apply h2
   apply h4
 
-case _ ih => -- spctor
+case _ As _ ih => -- spctor
   rw[Option.bind_eq_some_iff] at h; rcases h with ⟨h1, h2, h⟩
-  rw[Option.bind_eq_some_iff] at h; rcases h with ⟨h3, h4, h⟩; simp at h
+  rw[Option.bind_eq_some_iff] at h; rcases h with ⟨Ks, h4, h⟩; simp at h
   rcases h with ⟨h5, h⟩
-  rw[Option.bind_eq_some_iff] at h; rcases h with ⟨h6, h7, h⟩; simp at h
+  rw[Option.bind_eq_some_iff] at h; rcases h with ⟨Ts', h7, h⟩; simp at h
   rcases h with ⟨h8, h⟩
   rcases h8 with ⟨h9, h10⟩
   rcases h9 with ⟨h11, h12⟩
-  replace h4 := Vec.seq_sound h4
-  sorry
-case _ => -- openm
-  sorry
+  subst h10;
+  apply Typing.spctor (R := h1.2.2.2.snd) (Ts := h1.2.2.2.1) (Ks := Ks) (Ts' := Ts')
+  · sorry
+  · sorry
+  · apply Eq.symm h
+  · intro i; replace h4 := Vec.map_seq_sound _ h4 i; replace h4 := infer_kind_sound h4;
+    simp[instGetElem_Vec]; rw[Vec.to_get_elem Ks, Vec.to_get_elem As] at h4; apply h4
+  · intro i; replace h7 := Vec.seq_sound1 _ h7 i;
+    apply ih i; simp[instGetElem_Vec]; rw[Vec.to_get_elem] at h7; apply h7
+  · intro c e; cases e; apply h11
+  · intro h; cases h
+
+
+case _ As _ ih => -- openm
+  rw[Option.bind_eq_some_iff] at h; rcases h with ⟨h1, h2, h⟩
+  rw[Option.bind_eq_some_iff] at h; rcases h with ⟨Ks, h4, h⟩
+  simp at h; rcases h with ⟨h5, h⟩
+  rw[Option.bind_eq_some_iff] at h; rcases h with ⟨Ts', h7, h⟩
+  rw[Option.bind_eq_some_iff] at h; rcases h with ⟨h8, h9, h⟩
+  simp at h; rcases h with ⟨h10, h11⟩
+  rcases h10 with ⟨h10, e⟩; subst e
+  rcases h5 with ⟨h5, e⟩; subst e
+  apply Typing.spctor (R := h1.2.2.2.snd) (Ts := h1.2.2.2.1) (Ks := Ks) (Ts' := Ts')
+  · sorry
+  · sorry
+  · apply (Eq.symm h11)
+  · intro i; replace h4 := Vec.map_seq_sound _ h4 i; replace h4 := infer_kind_sound h4;
+    simp[instGetElem_Vec]; rw[Vec.to_get_elem Ks, Vec.to_get_elem As] at h4; apply h4
+  · intro i; replace h7 := Vec.seq_sound1 _ h7 i;
+    apply ih i; simp[instGetElem_Vec]; rw[Vec.to_get_elem] at h7; apply h7
+  · intro c e; cases e
+  · intro e i; cases e; replace h9 := Vec.map_seq_sound _ h9 i;
+    have lem := Vec.units h8 i; rw[lem] at h9
+    replace h9 := data_valid_sound _ h9; simp[instGetElem_Vec];
+    rw[Vec.to_get_elem] at h9; apply h9
+
+
 case _ m n ss ps ts smτs ih1 ih2 => -- match
   rw[Option.bind_eq_some_iff] at h; rcases h with ⟨S, h2, h⟩
   rw[Option.bind_eq_some_iff] at h; rcases h with ⟨h3, h4, h⟩
-  rw[Option.bind_eq_some_iff] at h; rcases h with ⟨h5, h6, h⟩
+  rw[Option.bind_eq_some_iff] at h; rcases h with ⟨ξ, h6, h⟩
   rw[Option.bind_eq_some_iff] at h; rcases h with ⟨h7, h8, h⟩
-  apply Typing.mtch (m := m) (n := n) (S := S.to)
-  sorry
-  sorry
-  intro i; replace h6 := Vec.seq_sound h6; replace h6 := h6 i; sorry
-  sorry
-  intro q qs; sorry
-  sorry
+  rw[Option.bind_eq_some_iff] at h; rcases h with ⟨h9, h10, h11⟩
+  apply Typing.mtch (m := m) (n := n) (S := S.to) (ξ := ξ.to)
+  · intro i; unfold smτs at h2; replace h2 := Vec.seq_sound1 _ h2;
+    apply ih1 i (T := S.to i) (h2 i);
+  · intro i; replace h4 := Vec.map_seq_sound _ h4 i;
+    have lem := Vec.units h3 i; rw[lem] at h4
+    apply data_valid_sound _ h4
+  · intro i; replace h6 := Vec.seq_sound1 _ h6 i;
+    apply pattern_binders_sound;
+    rw[<-Fun.Vec.to_iso (v := S)] at h6; apply h6
+  · intro i; replace ih2 := ih2 ξ;
+    replace ih2 := ih2 (T := T) i
+    rw[Vec.get_elem_indexing (vs := ξ)]
+    apply ih2
+    replace h10 := Vec.seq_sound2 _ h10 i;
+    replace h11 := Vec.get_elem_if_eq_sound h11 i
+    rw[<-Vec.get_elem_indexing] at h11; rw [h11] at h10; apply h10
+  · intro q qs; apply pattern_exhaustive_sound G q qs h8
 
+case _ ih1 ih2 => -- cast
+  rw[Option.bind_eq_some_iff] at h; rcases h with ⟨h1, h2, h⟩
+  rw[Option.bind_eq_some_iff] at h; rcases h with ⟨h3, h4, h⟩
+  rw[Option.bind_eq_some_iff] at h; rcases h with ⟨K, h6, h⟩
+  rw[Option.bind_eq_some_iff] at h; rcases h with ⟨h7, h8, h⟩
+  rw[Option.bind_eq_some_iff] at h; rcases h with ⟨h9, h10, h⟩
+  simp at h; rcases h with ⟨h10, h11⟩
+  subst h11; subst h10
+  replace h8 := Kind.base_kind_sound K h8; subst h8
+  replace h4 := Ty.is_eq_some_sound h4; subst h1
+  apply Typing.cast
+  · replace h6 := infer_kind_sound h6
+    apply h6
+  · apply ih1 h2
+  · apply ih2 h10
+  · rfl
 
-sorry
-sorry
-sorry
-sorry
+case _ ih => -- lam
+  rw[Option.bind_eq_some_iff] at h; rcases h with ⟨h1, h2, h⟩
+  rw[Option.bind_eq_some_iff] at h; rcases h with ⟨h3, h4, h⟩
+  rw[Option.bind_eq_some_iff] at h; rcases h with ⟨B, h6, h⟩
+  rw[Option.bind_eq_some_iff] at h; rcases h with ⟨h6, h7, h⟩
+  rw[Option.bind_eq_some_iff] at h; rcases h with ⟨h8, h9, h⟩
+  cases h;
+  replace h9 := Kind.base_kind_sound _ h9; subst h6
+  replace h4 := Kind.base_kind_sound _ h4; subst h1
+  apply Typing.lam
+  · apply infer_kind_sound h2
+  · apply ih h6
+
+case _ => -- refl
+  rw[Option.bind_eq_some_iff] at h; rcases h with ⟨h1, h2, h⟩
+  cases h
+  apply Typing.refl
+  · apply infer_kind_sound h2
+
+case _ ih => -- t •[T]
+  rw[Option.bind_eq_some_iff] at h; rcases h with ⟨h1, h2, h⟩
+  rw[Option.bind_eq_some_iff] at h; rcases h with ⟨h3, h4, h⟩
+  rw[Option.bind_eq_some_iff] at h; rcases h with ⟨h5, h6, h⟩
+  simp at h; rcases h with ⟨h6, h7⟩
+  subst h1; subst T
+  replace h6 := Ty.is_all_some_sound h6; subst h3
+  apply Typing.appt
+  · apply ih h4
+  · apply infer_kind_sound h2
+  · rfl
+
 sorry
 sorry
 sorry
